added EquivGeneralize

theories/Defun.v
@@ -1,5 +1,5 @@
 Require Import List PeanoNat.
-(*Require Import StateMachines.Plugin.*)
+Require Import StateMachines.Plugin.
 Import ListNotations.
 Set Universe Polymorphism.
 
@@ -20,8 +20,20 @@ Inductive t (eff : Type -> Type) (a : Type) :=
 Inductive effect : Type -> Type :=
 | getE : unit -> effect nat
 | putE : nat -> effect unit
-| skipE : unit -> effect unit.
+| skipE : forall T, unit -> effect T.
 
+
+Fixpoint seqt eff a (e1 : t eff unit) (e2 : t eff a) :=
+  match e1 with
+  | Pure _ _ => e2
+  | Eff ef prog => Eff ef (fun x => seqt (prog x) e2)
+  end.
+
+Fixpoint foreach eff a T (l : list T)(e : t eff a)(f : T -> t eff a -> t eff a) :=
+  match l with
+  | [] => e
+  | x::l' => f x (foreach l' e f)
+  end.
 
 Notation "n <- 'get' ; e" := (Eff (getE tt) (fun n => e)) (at level 100, right associativity).
 Notation "'put' n ; e" := (Eff (putE n) (fun _ => e)) (at level 100).
@@ -37,12 +49,12 @@ Definition ex1 : t effect unit:=
     put (1 + n);
     Pure _ tt.
 
-Definition step_range (state a : Type) :=
+Definition step_range (state : Type) :=
   option {ty : Set & (effect ty * (ty -> state))%type }.
 
 Open Scope type_scope.
 
-Inductive equiv (state a : Type)(step : state -> step_range state a) :
+Inductive equiv (state a : Type)(step : state -> step_range state) :
   state -> t effect a -> Prop :=
 | EquivEffGet :
     forall (current : state)(f : nat -> state)(prog : nat -> t effect a),
@@ -59,18 +71,25 @@ Inductive equiv (state a : Type)(step : state -> step_range state a) :
 | EquivEffSkip :
     forall (current : state)(f : unit -> state)(prog : unit -> t effect a),
       step current
-      = Some (existT _ _ (skipE tt, f)) ->
+      = Some (existT _ _ (skipE unit tt, f)) ->
       equiv step (f tt) (prog tt) ->
-      equiv step current (Eff (skipE tt) prog)
+      equiv step current (Eff (skipE unit tt) prog)
 | EquivPure :
     forall (current : state)(x : a),
       step current = None ->
       equiv step current (Pure _ x)
 | EquivStateSkip :
-    forall (current : state)(f : unit -> state)(e : t effect a),
+    forall (current : state)(T : Type)(f : T -> state)(e : t effect a),
       step current
-      = Some (existT _ _(skipE tt, f)) ->
-      equiv step (f tt) e ->
+      = Some (existT _ _(skipE T tt, f)) ->
+      (forall x:T, equiv step (f x) e) ->
+      equiv step current e
+| EquivGeneralize :
+    forall (current : state)(T : Type)(x0 : T)(f : T -> state)(e' : T -> t effect a) e,
+      step current
+      = Some (existT _ _ (skipE T tt, f)) ->
+      e' x0 = e ->
+      (forall x:T, equiv step (f x) (e' x)) ->
       equiv step current e.
 
 
@@ -109,12 +128,19 @@ Ltac ptr_to_step_f_aux ptr accum :=
 Ltac ptr_to_step_f ptr :=
   ptr_to_step_f_aux ptr open_constr:(fun f => f).
 
-
 Ltac curry_lhs :=
-  match goal with
-    |- ?f (_,_) = _ =>
-    let f' := open_constr:(prod_curry _) in
-    unify f f'; unfold prod_curry
+  lazymatch goal with
+    |- ?x = _ =>
+    let rec aux p :=
+        lazymatch p with
+        | ?f (_,_) =>
+          let f' := open_constr:(prod_curry _) in
+          unify f f'; unfold prod_curry
+        | ?p' _ =>
+          aux p'
+        end
+    in
+    aux x
   end.
 
 
@@ -122,7 +148,7 @@ Ltac curry_lhs :=
 Ltac pattern_rhs term :=
   match goal with
     |- _ = ?X =>
-    let x := fresh "x" in
+    let x := fresh in
     set (x := X); pattern term in x; subst x
   end.
 
@@ -156,9 +182,9 @@ Ltac unify_to_subterm_im t1 t2 :=
 Ltac env_subst env n m :=
   lazymatch env with
   | n => m
-  | (n,?x) => constr:((m,x))
-  | (?k,?x) => let x' := env_subst x n m in
-               constr:((k,x'))
+  | (?x,n) => constr:((x,m))
+  | (?x,?k) => let x' := env_subst x n m in
+               constr:((x',k))
   | _ => env
   end.
 
@@ -175,9 +201,8 @@ Ltac skip_to env nextptr :=
     context_of current env ptr;
     let step_f := ptr_to_step_f ptr in
     let ty_env := type of env in
-    let f := open_constr:(_  : ty_env -> step_range state a ) in
-    eapply (@EquivStateSkip _ _ (step_f f) (ptr env)
-                            (fun _ => nextptr))
+    let f := open_constr:(_  : ty_env -> step_range state) in
+    eapply (@EquivStateSkip _ _ (step_f f) (ptr env) _ nextptr)
   end.
 
 Ltac is_concr_nat n :=
@@ -197,11 +222,11 @@ Ltac derive env :=
       let env_f' :=
           lazymatch env with
           | tt => open_constr:(fun n:nat => n)
-          | _ => open_constr:(fun n:nat => (n,env))
+          | _ => open_constr:(fun n:nat => (env,n))
           end
       in
       let step_f := ptr_to_step_f ptr in
-      let f := open_constr:(_  : ty_env -> step_range state a ) in
+      let f := open_constr:(_  : ty_env -> step_range state) in
       let f' := open_constr:(_) in
       eapply (@EquivEffGet _ _ (step_f (f ||| f')) (ptr (inl env))
                            (fun n => ptr (inr (inl (env_f' n)))));
@@ -210,7 +235,7 @@ Ltac derive env :=
        intro n; derive constr:(env_f' n)]
     | Eff (putE ?n) ?e =>
       let step_f := ptr_to_step_f ptr in
-      let f  := open_constr:(_ : ty_env -> step_range state a) in
+      let f  := open_constr:(_ : ty_env -> step_range state) in
       lazymatch e with
       | (fun _ => Pure _ _) =>
         eapply (@EquivEffPut _ _ (step_f (f ||| (fun _ => None))) (ptr (inl env))
@@ -224,11 +249,11 @@ Ltac derive env :=
       end
     | (match ?m with | O => ?progO | S _ => ?progS end) =>
       let step_f := ptr_to_step_f ptr in
-      let f := open_constr:(_  : ty_env -> step_range state a ) in
+      let f := open_constr:(_  : ty_env -> step_range state) in
       let f' := open_constr:(_) in
       let env' := (eval simpl in env) in
       let env0 := env_subst env' m 0 in
-      eapply (@EquivStateSkip _ _ (step_f (f ||| f')) (ptr (inl env))
+      eapply (@EquivStateSkip _ _ (step_f (f ||| f')) (ptr (inl env)) unit
                               (fun _ => match m with
                                         | O =>
                                           ptr (inr (inl (inl env0)))
@@ -238,59 +263,203 @@ Ltac derive env :=
       [ unify_fun
       | let m' := fresh "m'" in
         destruct m as [|m'];
-        [ derive env0 | let envm' := env_subst env' m m' in derive envm' ]]
+        [ derive env0 | let envm' := env_subst env' m m' in derive envm' ]
+      ]
     | _ =>
       let p := leftmost prog in
-     (* tryif is_fix p then*)
-        (  skip_to env open_constr:(ptr (inr env));
-          [unify_fun|
-           skip_to env open_constr:(_);
-           [unify_fun|progress auto]])
+      tryif is_fix p then
+        (skip_to env open_constr:(fun _:unit => ptr (inr env));
+         intros;
+         [unify_fun
+         | skip_to env open_constr:(fun _:unit => _);
+           intros;
+           [unify_fun|progress repeat match goal with H : _ |- _ => refine (H _) end]])
         || (
           let step_f := ptr_to_step_f ptr in
-            let f := open_constr:(_  : ty_env -> step_range state a ) in
+          let f := open_constr:(_  : ty_env -> step_range state) in
+          let f' := open_constr:(_) in
+          let env' := (eval simpl in env) in
+          let m := match prog with _ ?k => k end in
+          let env0 := match type of m with
+                      | nat => env_subst env' m 0
+                      | list ?A => env_subst env' m (@nil A)
+                      end
+          in
+          let k := fresh "k" in
+          let rec generalize_args e tac :=
+              lazymatch e with
+              | ?e' m =>
+                lazymatch p with
+                | context[m] =>
+                  eapply (@EquivGeneralize _ _ (step_f (f ||| f')) (ptr (inl env)) _ m (fun k:nat => match m with
+                                                                                                   | O => ptr (inr (inl (inl (env0,k))))
+                                                                                                   | S m' => ptr (inr (inr (inl (_, k))))
+                                                                                                   end));
+                  [ unify_fun
+                  | match goal with
+                      |- ?e ?x = ?f ?x =>
+                      match eval pattern x in f with
+                        ?g _ => exact (eq_refl: e x = (fun y => g y x) x)
+                      end
+                    end
+                  | let m' := fresh "n'" in
+                  induction m as [|m'];
+                  intro k;
+                  simpl;
+                  [ tac env0 0
+                  | tac env' m' ]
+                  ]
+                | _ =>
+                  generalize_args e' tac
+                end
+              | ?e' ?x =>
+                eapply (@EquivGeneralize _ _ (step_f (f ||| f')) (ptr (inl env)) _ x (fun k:nat => match m with
+                                                                                                   | O => ptr (inr (inl (inl (env0,k))))
+                                                                                                   | S m' => ptr (inr (inr (inl (_, k))))
+                                                                                                   end));
+                [ unify_fun
+                | generalize x;
+                  intros;
+                  lazymatch goal with
+                    |- _ ?x = _ =>
+                    pattern_rhs x;
+                    try apply eq_refl
+                  | _ => idtac
+                  end
+                | let m' := fresh "n'" in
+                  induction m as [|m'];
+                  intro k;
+                  simpl;
+                  [ tac env0 0
+                  | tac env' m' ]
+                ]
+              | _ => idtac
+              end
+          in
+          generalize_args prog ltac:(fun env m' =>
+                                       let envm' := env_subst env' m m' in
+                                       derive (envm',k))
+        )
+     else fail 0
+    end
+  end.
+
+
+Ltac derive_step env :=
+  lazymatch goal with
+    |- @equiv ?state ?a ?step ?current ?prog =>
+    let ptr := open_constr:(?[ptr]) in
+    context_of current open_constr:(inl _) ptr;
+    let ty_env := type of env in
+    lazymatch prog with
+    | Eff (getE tt) _ =>
+      let env_f' :=
+          lazymatch env with
+          | tt => open_constr:(fun n:nat => n)
+          | _ => open_constr:(fun n:nat => (env,n))
+          end
+      in
+      let step_f := ptr_to_step_f ptr in
+      let f := open_constr:(_  : ty_env -> step_range state) in
+      let f' := open_constr:(_) in
+      eapply (@EquivEffGet _ _ (step_f (f ||| f')) (ptr (inl env))
+                           (fun n => ptr (inr (inl (env_f' n)))));
+      [unify_fun|
+       let n := fresh "n" in
+       intro n]
+    | Eff (putE ?n) ?e =>
+      let step_f := ptr_to_step_f ptr in
+      let f  := open_constr:(_ : ty_env -> step_range state a) in
+      lazymatch e with
+      | (fun _ => Pure _ _) =>
+        eapply (@EquivEffPut _ _ (step_f (f ||| (fun _ => None))) (ptr (inl env))
+                             (fun _ => ptr (inr env)));
+        [try unify_fun|eapply EquivPure; auto]
+      | _ =>
+        let f' := open_constr:(_) in
+        eapply (@EquivEffPut _ _ (step_f (f ||| f')) (ptr (inl env))
+                             (fun _ => ptr (inr (inl env))));
+        [unify_fun|]
+      end
+    | (match ?m with | O => ?progO | S _ => ?progS end) =>
+      let step_f := ptr_to_step_f ptr in
+      let f := open_constr:(_  : ty_env -> step_range state) in
+      let f' := open_constr:(_) in
+      let env' := (eval simpl in env) in
+      let env0 := env_subst env' m 0 in
+      eapply (@EquivStateSkip _ _ (step_f (f ||| f')) (ptr (inl env)) unit
+                              (fun _ => match m with
+                                        | O =>
+                                          ptr (inr (inl (inl env0)))
+                                        | S m' =>
+                                          ptr (inr (inr (@inl nat _ _)))
+                                        end));
+      [ unify_fun
+      | let m' := fresh "m'" in
+        destruct m as [|m']
+      ]
+    | _ =>
+      let p := leftmost prog in
+      tryif is_fix p then
+        (skip_to env open_constr:(fun _:unit => ptr (inr env));
+         intros;
+         [ unify_fun
+         | skip_to env open_constr:(fun _:unit => _);
+          intros;
+          [unify_fun|progress eauto]])
+        || (
+          let step_f := ptr_to_step_f ptr in
+            let f := open_constr:(_  : ty_env -> step_range state) in
             let f' := open_constr:(_) in
             let env' := (eval simpl in env) in
             let m := match prog with _ ?k => k end in
-            let env0 := env_subst env' m 0 in
-            eapply (@EquivStateSkip _ _ (step_f (f ||| f')) (ptr (inl env))
-                                    (fun _ => match m with
-                                              | O =>
-                                                ptr (inr (inl (inl env0)))
-                                              | S m' =>
-                                                ptr (inr (inr _))
-                                              end));
-            [ unify_fun
-            | let rec generalize_args e tac :=
-                  lazymatch e with
-                  | ?e' m => generalize_args e' tac
-                  | ?e' ?x =>
-                    tryif is_concr_nat x then
-                        let s := fresh "n" in
-                        generalize x at 1 as s;
-                        generalize_args e'
-                                        ltac:(fun env m' =>
-                                                intro s;
-                                                tac constr:((s,env)) m')
-                    else
-                      (generalize dependent x;
-                       generalize_args e' ltac:(fun env m' =>
-                                                  intro x;
-                                                  tac env m'))
-                  | _ =>
-                    let m' := fresh "n'" in
-                    induction m as [|m'];
-                    [ tac env0 0
-                    | tac env m'
-                    ]
-                  end
-              in
-              generalize_args prog ltac:(fun env m' =>
-                                           let envm' := env_subst env' m m' in
-                                           derive envm')
-            ]
+            let env0 := match type of m with
+                        | nat => env_subst env' m 0
+                        | list ?A => env_subst env' m (@nil A)
+                        end
+            in
+            
+          let rec generalize_args e tac :=
+              lazymatch e with
+              | ?e' m =>
+                lazymatch p with
+                | context[m] =>
+                  eapply (@EquivGeneralize _ _ (step_f (f ||| f')) (ptr (inl env)) _ m (fun k:nat => match m with
+                                                                                                   | O => ptr (inr (inl (inl (env0,k))))
+                                                                                                   | S m' => ptr (inr (inr (inl (_, k))))
+                                                                                                   end));
+                  [ unify_fun
+                  | match goal with
+                      |- ?e ?x = ?f ?x =>
+                      match eval pattern x in f with
+                        ?g _ => exact (eq_refl: e x = (fun y => g y x) x)
+                      end
+                    end
+                  |
+                  ]
+                | _ =>
+                  generalize_args e' tac
+                end
+              | ?e' ?x =>
+                eapply (@EquivGeneralize _ _ (step_f (f ||| f')) (ptr (inl env)) _ x (fun k:nat => match m with
+                                                                                                   | O => ptr (inr (inl (inl (env0,k))))
+                                                                                                   | S m' => ptr (inr (inr (inl (_, k))))
+                                                                                                   end));
+                [ unify_fun
+                | generalize x; try reflexivity
+                | let m' := fresh "n'" in
+                  induction m as [|m'];
+                  [ tac env0 0
+                  | tac env' m' ]
+                ]
+              | _ => idtac
+              end
+          in
+          generalize_args prog ltac:(fun env m' =>
+                                       let envm' := env_subst env' m m' in
+                                       idtac)
         )
-     (* else idtac*)
+     else idtac
     end
   end.
 
@@ -301,15 +470,13 @@ Definition ex : t effect unit :=
     put (n + n0 + n1);
     Pure _ tt.
 
-
-(*
-n <- get;
-a = 0;
-for 0..(n-1)
-  x <- get;
-  a = a + x;
-put a;
- *)
+Definition ex_derive :
+  {state & {step & {init | @equiv state _ step init ex}}}.
+Proof.
+  unfold ex.
+  repeat eexists.
+  derive tt.
+Defined.
 
 Fixpoint ex3' (a n : nat) : t effect unit :=
   match n with
@@ -317,16 +484,12 @@ Fixpoint ex3' (a n : nat) : t effect unit :=
   | S n' => x <- get; ex3' (x + a) n'
   end.
 
-Definition ex3 : t effect unit :=
-  n <- get; ex3' 5 n.
-
 Definition ex3'_derive :
   {state & {step & forall a n, { init | @equiv state _ step init (ex3' a n) }}}.
 Proof.
   unfold ex3'.
   repeat eexists.
-
-  derive (n,a).
+  derive (a,n).
 Defined.
 
 Eval cbv in projT1 ex3'_derive.
@@ -344,16 +507,75 @@ Definition ex3''_derive :
 Proof.
   unfold ex3'',ex3'.
   repeat eexists.
-
   derive tt.
 Defined.
 
-Set Printing Evars.
+
+Definition ex3 : t effect unit :=
+  n <- get; ex3' 5 n.
+
 Definition ex3_derive :
   {state & {step & {init | @equiv state _ step init ex3 }}}.
 Proof.
   unfold ex3, ex3'.
   repeat eexists.
-
   derive tt.
-  simpl.
+Defined.  
+
+Definition ex5 : t effect unit :=
+  n <- get;
+    (fix f m :=
+       match m with
+       | O => put n; Pure _ tt
+       | S m' => put n; f m'
+       end) n.
+
+Definition ex5_derive :
+  { state & { step & { init | @equiv state _ step init ex5 }}}.
+Proof.
+  unfold ex5.
+  repeat eexists.
+  derive tt.
+Defined.
+
+Eval cbv [ex5 ex5_derive sum_merge prod_curry projT1 projT2] in (projT1 (projT2 ex5_derive)).
+
+Definition double_loop : t effect unit :=
+  n <- get;
+    (fix f m :=
+       match m with
+       | O => put 0; Pure _ tt
+       | S m' =>
+         x <- get;
+           (fix g k :=
+              match k with
+              | O => f m'
+              | S k' => put 1; g k'
+              end) x
+       end) n.
+
+Definition double_loop_derive :
+  {state & {step & {init | @equiv state _ step init double_loop}}}.
+Proof.
+  unfold double_loop.
+  repeat eexists.
+  derive tt.
+  derive_step n.
+  
+Defined.
+
+Definition ex_list : t effect unit :=
+  n <- get;
+    (fix f l m :=
+       match m with
+       | O => put 0; Pure _ tt
+       | S m' =>
+         x <- get;
+           (fix g l' :=
+              match l' with
+              | [] => f (x::l) m'
+              | a::rest =>
+                put a;
+                  g rest
+              end) l
+       end) [] n.
